Remove HandshakeMessages.valid_hs_msg, do not depend on protocol version
"Absolute" validity conditions that do not depend on the protocol version
are now integrated directly into the definition of handshake messages.

"Relative" validity conditions that depend on the protocol version should
appear only at the level of HandshakeLog: such conditions are also more
global, they specifically constrain the shape of the whole message
transcript.

src/tls/HandshakeLog.fst
@@ -89,42 +89,8 @@ let print_hsl (hsl:erased_transcript) : Tot bool =
     IO.debug_print_string ("Current log: " ^ s)
     else false
 
-(* TODO: move to something like List.GTot *)
-let rec gforall_list_to_list_refined
-  (#a: Type)
-  (f: (a -> GTot bool))
-  (l: list a { gforall f l } )
-: Tot (l': list (x: a {f x}))
-= match l with
-  | [] -> []
-  | x :: q -> x :: gforall_list_to_list_refined f q
-
-let rec valid_transcript_to_list_valid_hs_msg_aux
-  (v: option protocolVersion)
-  (l: list hs_msg { gforall (valid_hs_msg_prop v) l } )
-: Tot (list (valid_hs_msg v))
-=
-(* FIXME: WHY WHY WHY can this not be defined as:
-   gforall_list_to_list_refined (valid_hs_msg_prop v) l
-*)
-  match l with
-  | [] -> []
-  | a :: q -> a :: valid_transcript_to_list_valid_hs_msg_aux v q
-
-let rec valid_transcript_to_list_valid_hs_msg_aux_inj
-  (v: option protocolVersion)
-  (l1: list hs_msg { gforall (valid_hs_msg_prop v) l1 } )
-  (l2: list hs_msg { gforall (valid_hs_msg_prop v) l2 } )
-: Lemma
-  (requires (valid_transcript_to_list_valid_hs_msg_aux v l1 == valid_transcript_to_list_valid_hs_msg_aux v l2))
-  (ensures (l1 == l2))
-= match l1, l2 with
-  | _ :: q1, _ :: q2 -> valid_transcript_to_list_valid_hs_msg_aux_inj v q1 q2
-  | _ -> ()
-
 let transcript_bytes l =
-  let v = transcript_version l in
-  handshakeMessagesBytes v (valid_transcript_to_list_valid_hs_msg_aux v l)
+  handshakeMessagesBytes l
 
 #set-options "--z3rlimit 64"
 
@@ -133,23 +99,7 @@ let transcript_format_injective ms0 ms1 =
   : Lemma
     (requires (Seq.equal (transcript_bytes ms0) (transcript_bytes ms1)))
     (ensures (ms0 == ms1))
-  = match ms0 with
-    | [] -> ()
-    | ClientHello ch0 :: q0 ->
-      let v = transcript_version ms0 in
-      let (ClientHello ch1 :: q1) = ms1 in
-      let v1 = transcript_version ms1 in
-      let l0 = handshakeMessagesBytes v (valid_transcript_to_list_valid_hs_msg_aux v q0) in
-      let l1 = handshakeMessagesBytes v1 (valid_transcript_to_list_valid_hs_msg_aux v1 q1) in
-      clientHelloBytes_is_injective_strong ch0 l0 ch1 l1;
-      begin match q0 with
-      | [] -> ()
-      | ServerHello sh0 :: q0' ->
-        let (ServerHello sh1 :: q1') = q1 in
-        serverHelloBytes_is_injective_strong sh0 (handshakeMessagesBytes v (valid_transcript_to_list_valid_hs_msg_aux v q0')) sh1 (handshakeMessagesBytes v1 (valid_transcript_to_list_valid_hs_msg_aux v1 q1'));
-        handshakeMessagesBytes_is_injective v (valid_transcript_to_list_valid_hs_msg_aux v ms0) (valid_transcript_to_list_valid_hs_msg_aux v ms1);
-        valid_transcript_to_list_valid_hs_msg_aux_inj v ms0 ms1
-      end
+  = handshakeMessagesBytes_is_injective ms0 ms1
   in
   Classical.move_requires f ()
 
@@ -291,7 +241,7 @@ let getHash #ha (LOG #reg st) =
 let send l m =
   trace ("emit "^HandshakeMessages.string_of_handshakeMessage m);
   let st = !l in
-  let mb = handshakeMessageBytes st.pv m in
+  let mb = handshakeMessageBytes m in
   let h : hashState st.transcript (st.parsed @ [m]) =
     match st.hashes with
     | FixedHash a acc hl ->
@@ -323,7 +273,7 @@ let hash_tag_truncated #a l len =
 let send_tag #a l m =
   trace ("emit "^HandshakeMessages.string_of_handshakeMessage m^" and hash");
   let st = !l in
-  let mb = handshakeMessageBytes st.pv m in
+  let mb = handshakeMessageBytes m in
   let (h,tg) : (hashState st.transcript (st.parsed @ [m]) * anyTag) =
     match st.hashes with
     | FixedHash a' acc hl ->
@@ -345,7 +295,7 @@ let send_tag #a l m =
 
 let send_CCS_tag #a l m cf =
   let st = !l in
-  let mb = handshakeMessageBytes st.pv m in
+  let mb = handshakeMessageBytes m in
   let (h,tg) : (hashState st.transcript (st.parsed @ [m]) * anyTag) =
     match st.hashes with
     | FixedHash a acc hl ->
